code/ecdsa/Hacl.Impl.EC.DH.fst
@@ -65,7 +65,7 @@ let ecp256dh_i c l result scalar =
 
 [@ (Comment "  This code is not side channel resistant on pubKey")]
 inline_for_extraction noextract
-val _ecp256dh_r: #c: curve 
+val _ecp256dh_r_public: #c: curve 
   -> #l: ladder 
   -> result: point c
   -> pubKey: point c
@@ -90,14 +90,71 @@ val _ecp256dh_r: #c: curve
 	r == true) end))
 
 
-let _ecp256dh_r #c #l result pubKey scalar =
+let _ecp256dh_r_public #c #l result pubKey scalar =
     let h0 = ST.get() in 
   push_frame();
     let len = getCoordinateLenU64 c in 
     let tempBuffer = create (size 20 *! len) (u64 0) in
     let h1 = ST.get() in 
     Hacl.Impl.P.PointAdd.Aux.lemma_getZ_noChangeInState c h0 h1 pubKey;
-  let publicKeyCorrect = verifyQValidCurvePoint #c #l pubKey tempBuffer in 
+  let publicKeyCorrect = verifyQValidCurvePoint_public #c #l pubKey tempBuffer in 
+  if publicKeyCorrect then
+    begin
+        let h2 = ST.get() in 
+	Hacl.Impl.P.PointAdd.Aux.lemma_coord_eval c h0 h2 pubKey;
+	scalarMultiplication #c #MUT #l pubKey result scalar tempBuffer; 
+	  let h3 = ST.get() in 
+	let flag = isPointAtInfinityPrivate #c result in 
+	pop_frame();
+	  let h4 = ST.get() in 
+	  Hacl.Impl.P.PointAdd.Aux.lemma_coord_eval c h3 h4 result;
+	let open Hacl.Impl.EC.LowLevel.RawCmp in 
+	unsafe_bool_of_u64 flag
+    end
+  else
+    begin
+      pop_frame();
+	let h2 = ST.get() in 
+      Hacl.Impl.P.PointAdd.Aux.lemma_coord_eval c h0 h2 result;
+      false
+    end
+
+
+
+inline_for_extraction noextract
+val _ecp256dh_r_private: #c: curve 
+  -> #l: ladder 
+  -> result: point c
+  -> pubKey: point c
+  -> scalar: scalar_t #MUT #c -> 
+  Stack bool
+  (requires fun h -> live h result /\ live h pubKey /\ live h scalar /\ 
+     LowStar.Monotonic.Buffer.all_disjoint [loc pubKey;  loc scalar; loc result] /\ (
+    let pk = as_nat c h (getX pubKey), as_nat c h (getY pubKey), as_nat c h (getZ pubKey) in 
+    ~ (isPointAtInfinity pk) /\ as_nat c h (getZ pubKey) == 1 /\
+    as_nat c h (getX result) == 0 /\ as_nat c h (getY result) == 0 /\ as_nat c h (getZ result) == 0))
+  (ensures fun h0 r h1 -> modifies (loc result |+| loc pubKey) h0 h1 /\ point_eval c h1 result /\ (
+    let pk = as_nat c h0 (getX pubKey), as_nat c h0 (getY pubKey), as_nat c h0 (getZ pubKey) in 
+    let x3, y3, z3 = point_as_nat c h1 result in
+    if not (verifyQValidCurvePointSpec #c pk) then
+      r = false /\ x3 == 0 /\ y3 == 0
+    else begin
+      let xN, yN, zN = scalar_multiplication #c (as_seq h0 scalar) pk in
+      xN == x3 /\ yN == y3 /\ zN == z3 /\ (
+      if isPointAtInfinity (xN, yN, zN) then
+	r == false
+      else
+	r == true) end))
+
+
+let _ecp256dh_r_private #c #l result pubKey scalar =
+    let h0 = ST.get() in 
+  push_frame();
+    let len = getCoordinateLenU64 c in 
+    let tempBuffer = create (size 20 *! len) (u64 0) in
+    let h1 = ST.get() in 
+    Hacl.Impl.P.PointAdd.Aux.lemma_getZ_noChangeInState c h0 h1 pubKey;
+  let publicKeyCorrect = verifyQValidCurvePoint_private #c #l pubKey tempBuffer in 
   if publicKeyCorrect then
     begin
         let h2 = ST.get() in 
@@ -128,7 +185,7 @@ let lemma_zero_point_zero_coordinates c h p =
   Hacl.Impl.P.PointAdd.Aux.lemma_point_eval_if_zero c p h
 
 inline_for_extraction noextract
-val ecp256_dh_r_: #c: curve -> #l: ladder -> result: pointAffine8 c 
+val ecp256_dh_r_public_: #c: curve -> #l: ladder -> result: pointAffine8 c 
   -> pubKey: pointAffine8 c 
   -> scalar: scalar_t #MUT #c
   -> pkF: point c
@@ -145,18 +202,46 @@ val ecp256_dh_r_: #c: curve -> #l: ladder -> result: pointAffine8 c
     let resultX, resultY = as_seq h1 (getXAff8 result), as_seq h1 (getYAff8 result) in 
     r == flag /\ resultX == pointX /\ resultY == pointY))
 
-let ecp256_dh_r_ #c #l result pubKey scalar pkF rF = 
+let ecp256_dh_r_public_ #c #l result pubKey scalar pkF rF = 
     let h0 = ST.get() in 
   toFormPoint pubKey pkF; 
     let h1 = ST.get() in 
   Hacl.Impl.P.PointAdd.Aux.lemma_coord_eval c h0 h1 rF; 
-  let flag = _ecp256dh_r #c #l rF pkF scalar in 
+  let flag = _ecp256dh_r_public #c #l rF pkF scalar in 
+  fromFormPoint rF result; 
+  flag
+
+
+inline_for_extraction noextract
+val ecp256_dh_r_private_: #c: curve -> #l: ladder -> result: pointAffine8 c 
+  -> pubKey: pointAffine8 c 
+  -> scalar: scalar_t #MUT #c
+  -> pkF: point c
+  -> rF: point c ->
+  Stack bool
+  (requires fun h -> live h result /\ live h pubKey /\ live h scalar /\ live h pkF /\ live h rF /\
+    disjoint pubKey pkF /\ point_eval c h rF /\ disjoint rF result /\
+    LowStar.Monotonic.Buffer.all_disjoint [loc rF; loc pkF; loc scalar] /\
+    as_nat c h (getX rF) == 0 /\ as_nat c h (getY rF) == 0 /\ as_nat c h (getZ rF) == 0
+  )
+  (ensures fun h0 r h1 -> modifies (loc result |+| loc pkF |+| loc rF) h0 h1 /\ (
+    let pubKeyX, pubKeyY = getXAff8 pubKey, getYAff8 pubKey in
+    let pointX, pointY, flag = ecp256_dh_r #c (as_seq h0 pubKeyX) (as_seq h0 pubKeyY) (as_seq h0 scalar) in
+    let resultX, resultY = as_seq h1 (getXAff8 result), as_seq h1 (getYAff8 result) in 
+    r == flag /\ resultX == pointX /\ resultY == pointY))
+
+let ecp256_dh_r_private_ #c #l result pubKey scalar pkF rF = 
+    let h0 = ST.get() in 
+  toFormPoint pubKey pkF; 
+    let h1 = ST.get() in 
+  Hacl.Impl.P.PointAdd.Aux.lemma_coord_eval c h0 h1 rF; 
+  let flag = _ecp256dh_r_public #c #l rF pkF scalar in 
   fromFormPoint rF result; 
   flag
 
 
 
-let ecp256dh_r #c #l result pubKey scalar =
+let ecp256dh_r_public #c #l result pubKey scalar =
   let h0 = ST.get() in 
   push_frame();
     let len = getCoordinateLenU64 c in 
@@ -167,7 +252,24 @@ let ecp256dh_r #c #l result pubKey scalar =
 
     lemma_create_zero_buffer #U64 (3 * v len) c;
     lemma_zero_point_zero_coordinates c h1 rF;
-  let flag = ecp256_dh_r_ #c #l result pubKey scalar pkF rF in 
+  let flag = ecp256_dh_r_public_ #c #l result pubKey scalar pkF rF in 
+
+  pop_frame();
+  flag
+
+
+let ecp256dh_r_private #c #l result pubKey scalar =
+  let h0 = ST.get() in 
+  push_frame();
+    let len = getCoordinateLenU64 c in 
+
+    let rF = create (size 3 *! len) (u64 0) in
+    let pkF = create (size 3 *! len) (u64 0) in
+    let h1 = ST.get() in 
+
+    lemma_create_zero_buffer #U64 (3 * v len) c;
+    lemma_zero_point_zero_coordinates c h1 rF;
+  let flag = ecp256_dh_r_private_ #c #l result pubKey scalar pkF rF in 
 
   pop_frame();
   flag
